Restructure

TheoremsAboutAlgorithms/Partitions/WithFinset/Split/Basic.lean
@@ -62,380 +62,6 @@ def insertEmpty {n : ℕ} (split : Split n) : Split n
 --     sorry
 
 ------------------------------------------------------------------------------------------------------------------------
---                          Bijections between split₀ and split.insertLastAt targetCell                               --
-------------------------------------------------------------------------------------------------------------------------
-
--- WIP (I)
-
--- What we want and define here are functions `f` and `g` (which will have more descriptive names below) such that
---
---    `f : split → split.insertLastAt targetCell`
---    `g : split.insertLastAt targetCell → split`
---
--- and `f ∘ g = id` and `g ∘ f = id`. We want to define them as follows:
---
---    `f := if cell = targetCell then cell.insertLast else cell.castSucc`
---    `g := if cell = targetCell.insertLast then targetCell else cell.castPred`
---
--- To do that we need an assumption `{Fin.last _} ∉ split.insertLastAt targetCell` to be able to define `g` as above,
--- because that has the preimage `∅` which we can't include in the domain of `f` (and therefore also not in the codomain
--- of `g`).
---
--- TODO: See in the usage later if that is what we actually need. Maybe we can `split.insertEmpty` work as domain of `f`
---       as codomain of `g` as well.
-
--- TODO:
---    * Prove that f and g are inverses
---    * Prove other useful stuff
---    * Theorem names and naming in general in this section are lacking, improve them!
-
--- TODO: Make this a section and define all the common implicit arguments (`n, split, targetCell`) at the top
-theorem insertLast_mem_insertLastAt_of_eq
-    {n : ℕ}
-    {split : Split n}
-    {targetCell cell : Cell n}
-    (cell_eq_targetCell : cell = targetCell)
-  : cell.insertLast ∈ split.insertLastAt targetCell := by
-    simp [insertLastAt]
-    left
-    rw [cell_eq_targetCell]
-
--- TODO: How can we make this anonymous so it can be found implicitly if we have the equality hypothesis?
---       Maybe this resource can help find the answer:
---        https://leanprover-community.github.io/mathlib4_docs/Init/Coe.html
---
---      Maybe `#print toInsertLastAt` can help us find the answer.
-instance CoeDepInsertLastInsertLastAtOfEq
-    {n : ℕ}
-    {split : Split n}
-    {targetCell cell : Cell n}
-    (cell_eq_targetCell : cell = targetCell)
-  : CoeDep (Cell (n + 1)) (cell.insertLast) (split.insertLastAt targetCell) where
-    coe := by
-      use cell.insertLast
-      exact insertLast_mem_insertLastAt_of_eq cell_eq_targetCell
-
--- We can't have `cell : split.insertEmpty`, because `Cell.castSucc ∅` is not in fact in `split.insertLastAt`. We do
--- however want to use this in the situation where `split` is a partition meaning that `∅ ∉ split`. We only use
--- `partitions.insertEmpty` there the have a target for the to create `{Fin.last _}`. We probably do not need to have
--- `insertEmptyToInsertLastAt` to go from `partition.insertEmpty` but can use just `partition` as the domain. We handle
--- the case where `cell = ∅` separately.
-theorem castSucc_mem_insertLastAt_of_ne
-    {n : ℕ}
-    {split : Split n}
-    {targetCell : Cell n}
-    {cell : split}
-    (cell_ne_targetCell : ↑cell ≠ targetCell)
-  : Cell.castSucc cell ∈ split.insertLastAt targetCell := by
-    simp [insertLastAt, castSucc, Cell.castSuccEmbedding, Cell.castSucc]
-    right
-    assumption
-
--- TODO: How can we make this anonymous (like above)?
-instance CoeDepCastSuccInsertLastAtOfNe
-    {n : ℕ}
-    {split : Split n}
-    {targetCell : Cell n}
-    {cell : split}
-    (cell_ne_targetCell : ↑cell ≠ targetCell)
-  : CoeDep (Cell (n + 1)) (Cell.castSucc cell) (split.insertLastAt targetCell) where
-    coe := by
-      use Cell.castSucc cell
-      exact castSucc_mem_insertLastAt_of_ne cell_ne_targetCell
-
-def upward
-    {n : ℕ}
-    {split : Split n}
-    {targetCell : Cell n}
-    (cell : split)
-  : split.insertLastAt targetCell :=
-    if h : cell = targetCell
-    -- CoeDep.coe.{u, v} {α : Sort u} (x✝ : α) {β : Sort v} [self : CoeDep α x✝ β] : β
-    -- then CoeDep.coe _ (Cell.castSucc cell) _ (CoeDepInsertLastInsertLastAtOfEq h)
-    then (CoeDepInsertLastInsertLastAtOfEq h).coe
-    else (CoeDepCastSuccInsertLastAtOfNe h).coe
-
--- TODO: Naming feels pretty imprecise here
-theorem ne_last_of_ne_insertLast_of_mem
-    {n : ℕ}
-    {split : Split n}
-    {targetCell : Cell n}
-    {cell : split.insertLastAt targetCell}
-    (cell_ne_targetCell_insertLast : ↑cell ≠ targetCell.insertLast)
-    (x : ↑cell)
-  : ↑x ≠ Fin.last n := by
-    have cell_mem_insertLastAt := cell.property
-    simp [insertLastAt] at cell_mem_insertLastAt
-    cases cell_mem_insertLastAt with
-      | inl _ => contradiction
-      | inr cell_mem_castSucc =>
-        apply Decidable.byContradiction
-        intro x_eq_last
-        simp at x_eq_last
-        have last_mem_cell : Fin.last n ∈ (cell : Cell (n + 1)) := by
-          have := x.property;
-          rw [x_eq_last] at this;
-          exact this
-        have last_not_mem_cell := last_not_mem_of_mem_castSucc cell_mem_castSucc
-        contradiction
-
--- TODO: Naming feels pretty imprecise here
-theorem ne_last_of_ne_insertLast
-    {n : ℕ}
-    {split : Split n}
-    {targetCell : Cell n}
-    {cell : split.insertLastAt targetCell}
-    (cell_ne_targetCell_insertLast : ↑cell ≠ targetCell.insertLast)
-  : ∀ x ∈ (cell : Cell (n + 1)), ↑x ≠ Fin.last n := by
-    intro x x_mem_cell
-    exact ne_last_of_ne_insertLast_of_mem cell_ne_targetCell_insertLast ⟨x, x_mem_cell⟩
-
-theorem mem_castSucc_of_ne_targetCell_of_mem_castSucc_erase_targetCell
-    {n : ℕ}
-    {split : Split n}
-    {targetCell : Cell n}
-    {cell : Cell (n + 1)}
-    (cell_mem_castSucc_erase_targetCell : cell ∈ (split.erase targetCell |> castSucc))
-  : cell ∈ split.castSucc := by
-      simp [castSucc, Cell.castSuccEmbedding] at *
-      obtain ⟨_, cell', _, _⟩ := cell_mem_castSucc_erase_targetCell
-      use cell'
-
--- cell'_mem_split : cell' ∈ split
--- castSucc_cell'_eq_cell : Cell.castSucc cell' = ↑cell
--- ⊢ Cell.castPred ↑cell _ ∈ split
-theorem castPred_mem_split_of_mem_split_of_castSucc_eq_of_last_not_mem
-    {n : ℕ}
-    {split : Split n}
-    {x : Cell n}
-    {y : Cell (n + 1)}
-    (x_mem_split : x ∈ split)
-    (castSucc_x_eq_y : Cell.castSucc x = y)
-    (last_not_mem_y : ∀ f ∈ y, f ≠ Fin.last _)
-  : Cell.castPred y last_not_mem_y ∈ split := by
-    -- See https://proofassistants.stackexchange.com/a/1063 for why we use `subst` here
-    rw [Cell.castPred_y_eq_x_of_castSucc_x_eq_y_of_forall_mem_y_ne_last castSucc_x_eq_y last_not_mem_y]
-    exact x_mem_split
-
-theorem castPred_mem_of_ne_insertLast_of_mem_castSucc
-    {n : ℕ}
-    {split : Split n}
-    {targetCell : Cell n}
-    {cell : split.insertLastAt targetCell}
-    (cell_ne_insertLast_targetCell : ↑cell ≠ targetCell.insertLast)
-    (cell_mem_castSucc : ↑cell ∈ split.castSucc)
-  : (Cell.castPred cell) (ne_last_of_ne_insertLast cell_ne_insertLast_targetCell) ∈ split := by
-    simp [castSucc, Cell.castSuccEmbedding] at cell_mem_castSucc
-    obtain ⟨cell', cell'_mem_split, castSucc_cell'_eq_cell⟩ := cell_mem_castSucc
-    -- We use the helper because `rw` and `subst` do not work here (probably because we're coercing `cell` via `↑cell`)
-    apply castPred_mem_split_of_mem_split_of_castSucc_eq_of_last_not_mem cell'_mem_split castSucc_cell'_eq_cell
-
-theorem castPred_mem_of_mem_insertLastAt_of_ne_targetCell
-    {n : ℕ}
-    {split : Split n}
-    {targetCell : Cell n}
-    {cell : split.insertLastAt targetCell}
-    (cell_ne_insertLast_targetCell : ↑cell ≠ targetCell.insertLast)
-  : (Cell.castPred cell) (ne_last_of_ne_insertLast cell_ne_insertLast_targetCell) ∈ split := by
-    have cell_mem_insertLastAt := cell.property
-    simp [insertLastAt] at cell_mem_insertLastAt
-    cases cell_mem_insertLastAt with
-      | inl cell_eq_targetCell_insertLast => contradiction
-      | inr cell_mem_castSucc =>
-        apply castPred_mem_of_ne_insertLast_of_mem_castSucc cell_ne_insertLast_targetCell
-        exact mem_castSucc_of_ne_targetCell_of_mem_castSucc_erase_targetCell cell_mem_castSucc
-
-instance CoeDepCastPredOfNeInsertLast
-    {n : ℕ}
-    {split : Split n}
-    {targetCell : Cell n}
-    {cell : split.insertLastAt targetCell}
-    (cell_ne_insertLast_targetCell : ↑cell ≠ targetCell.insertLast)
-  : CoeDep (Cell n) ((Cell.castPred cell) (ne_last_of_ne_insertLast cell_ne_insertLast_targetCell)) split where
-    coe := by
-      use (Cell.castPred cell) (ne_last_of_ne_insertLast cell_ne_insertLast_targetCell)
-      exact castPred_mem_of_mem_insertLastAt_of_ne_targetCell cell_ne_insertLast_targetCell
-
--- TODO: This should probably be defined for `cell ≠ {Fin.last _}`, we just handle that case differently, so we have the
---       codomain equal to `toInsertLastAt`'s domain
-def downward
-    {n : ℕ}
-    (split : Split n)
-    (targetCell : split)
-    (cell : split.insertLastAt targetCell)
-  : split :=
-    if h : cell = Cell.insertLast (targetCell : Cell n)
-    then targetCell
-    else (CoeDepCastPredOfNeInsertLast h).coe
-
-theorem castPred_x_mem_split_of_mem_split_of_castSucc_eq
-    {n : ℕ}
-    {split : Split n}
-    {x' : Cell n}
-    {x : Cell (n + 1)}
-    (x'_mem_split : x' ∈ split)
-    (castSucc_x'_eq_x : Cell.castSucc x' = x)
-    -- TODO: Better api for the precondition, maybe as a predicate?
-    (castPred_x_preCond : ∀ f ∈ x, f ≠ Fin.last _ := by simp)
-  : Cell.castPred x castPred_x_preCond ∈ split := by
-    subst x
-    simp [Cell.castPred_castSucc_eq]
-    exact x'_mem_split
-
--- Surjectivity
-theorem upward_surjective
-    {n : ℕ}
-    {split : Split n}
-    (targetCell : split)
-  : Function.Surjective (@upward _ split targetCell) := by
-    intro x
-    simp [upward]
-    -- TODO: Make this work
-    -- TODO: Find a way we can use better notation than the explicit long instance name
-    -- let y := (@CoeDepInsertLastInsertLastAtOfEq n _ _ ).coe
-    cases Decidable.eq_or_ne x (CoeDepInsertLastInsertLastAtOfEq rfl).coe with
-      | inl x_eq_coe_insertLast_targetCell =>
-        exists targetCell
-        exists targetCell.property
-        split
-        · exact x_eq_coe_insertLast_targetCell.symm
-        · contradiction
-      | inr x_ne_coe_insertLast_targetCell =>
-        have x_val_ne_insertLast_targetCell : (x : Cell (n + 1)) ≠ Cell.insertLast ↑targetCell := by
-          simp [CoeDep.coe] at *
-          intro x_val_eq_insertLast_targetCell
-          have : x = (CoeDepInsertLastInsertLastAtOfEq rfl).coe := by
-            apply @Subtype.eq _ _ x _
-            exact x_val_eq_insertLast_targetCell
-          contradiction
-        -- If we use this (instead of writing out the verbose expression), this makes `castPred_h_x` appear everywhere
-        -- we would otherwise have `_` in the proof state which is ugly
-        -- let castPred_h_x := (ne_last_of_ne_insertLast x_val_ne_insertLast_targetCell)
-        -- TODO: How can we make it that we put this into the context and it is found implicitly?
-        exists Cell.castPred x (ne_last_of_ne_insertLast x_val_ne_insertLast_targetCell)
-        have castPred_x_val_mem_split : Cell.castPred x (ne_last_of_ne_insertLast x_val_ne_insertLast_targetCell) ∈ split := by
-          have x_val_mem_insertLastAt := x.property
-          simp [insertLastAt, x_val_ne_insertLast_targetCell, castSucc, Cell.castSuccEmbedding]
-            at x_val_mem_insertLastAt
-          obtain ⟨_, x', x'_mem_split, castSucc_x'_eq_x_val⟩ := x_val_mem_insertLastAt
-          exact castPred_x_mem_split_of_mem_split_of_castSucc_eq x'_mem_split castSucc_x'_eq_x_val _
-        exists castPred_x_val_mem_split
-        split
-        · case _ castPred_x_val_eq_targetCell_val =>
-          have x_val_mem_insertLastAt := x.property
-          simp [insertLastAt, x_val_ne_insertLast_targetCell, castSucc, Cell.castSuccEmbedding]
-            at x_val_mem_insertLastAt
-          obtain ⟨x_val_ne_castSucc_targetCell, _⟩ := x_val_mem_insertLastAt
-          have := Cell.eq_castSucc_of_castPred_eq _ castPred_x_val_eq_targetCell_val
-          contradiction
-        · case _ castPred_x_val_ne_insertLast_targetCell =>
-          simp [CoeDep.coe]
-          apply Subtype.eq
-          simp [Cell.castSucc_castPred_eq]
-
--- Inverses
-
-theorem left_inverse_downward_upward
-    {n : ℕ}
-    {split : Split n}
-    (targetCell : split)
-  : Function.LeftInverse (@downward _ split targetCell) (@upward _ split targetCell) := by
-    intro x
-    simp [upward, downward]
-    split
-    · case _ x_eq_targetCell =>
-      split
-      · apply Subtype.eq
-        exact x_eq_targetCell.symm
-      · case _ insertLast_x_ne_insertLast_targetCell =>
-        simp [CoeDep.coe] at insertLast_x_ne_insertLast_targetCell
-        -- TODO: There has to be a better way to get f x = f y from x = y
-        have : Cell.insertLast ↑x = Cell.insertLast (targetCell : Cell n) := by
-          have : Cell.insertLast ↑x = Cell.insertLast (x : Cell n) := by rfl
-          rw (config := {occs := .pos [2]}) [x_eq_targetCell] at this
-          exact this
-        contradiction
-    · case _ x_ne_targetCell_insertLast =>
-      split
-      · case _ castSucc_x_eq_insertLast_targetCell =>
-        simp [CoeDep.coe] at castSucc_x_eq_insertLast_targetCell
-        have := Cell.castSucc_x_ne_insertLast_y (x : Cell n) (targetCell : Cell n)
-        contradiction
-      · case _ castSucc_x_ne_insertLast_targetCell =>
-        simp [CoeDep.coe, x_ne_targetCell_insertLast]
-        apply Subtype.eq
-        simp
-        apply Cell.castPred_y_eq_x_of_castSucc_x_eq_y_of_forall_mem_y_ne_last rfl
-
-theorem right_inverse_downward_upward
-    {n : ℕ}
-    {split : Split n}
-    (targetCell : split)
-  : Function.RightInverse (@downward _ split targetCell) (@upward _ split targetCell) := by
-    apply Function.LeftInverse.rightInverse_of_surjective
-    · apply left_inverse_downward_upward
-    · apply upward_surjective
-
-theorem left_inverse_upward_downward
-    {n : ℕ}
-    {split : Split n}
-    (targetCell : split)
-  : Function.LeftInverse (@upward _ split targetCell) (@downward _ split targetCell) := by
-    apply Function.RightInverse.leftInverse
-    apply right_inverse_downward_upward
-
-theorem right_inverse_upward_downward
-    {n : ℕ}
-    {split : Split n}
-    (targetCell : split)
-  : Function.RightInverse (@upward _ split targetCell) (@downward _ split targetCell) := by
-    apply Function.LeftInverse.rightInverse
-    apply left_inverse_downward_upward
-
-theorem upward_injective
-    {n : ℕ}
-    {split : Split n}
-    (targetCell : split)
-  : Function.Injective (@upward _ split targetCell)
-    := Function.LeftInverse.injective (left_inverse_downward_upward targetCell)
-
-theorem upward_bijective
-    {n : ℕ}
-    {split : Split n}
-    (targetCell : split)
-  : Function.Bijective (@upward _ split targetCell) := by
-    constructor
-    · apply upward_injective
-    · apply upward_surjective
-
-theorem downward_bijective
-    {n : ℕ}
-    {split : Split n}
-    (targetCell : split)
-  : Function.Bijective (@downward _ split targetCell) := by
-    apply Function.bijective_iff_has_inverse.mpr
-    exists upward
-    constructor
-    · apply left_inverse_upward_downward
-    · apply right_inverse_upward_downward
-
--- Injectivity, embeddings
-
-def upwardEmbedding
-    {n : ℕ}
-    {split : Split n}
-    (targetCell : split)
-  : Function.Embedding split (split.insertLastAt targetCell) :=
-    ⟨upward, upward_injective targetCell⟩
-
-def downwardEmbedding
-    {n : ℕ}
-    {split : Split n}
-    (targetCell : split)
-  : Function.Embedding (split.insertLastAt targetCell) split :=
-    ⟨downward split targetCell, (downward_bijective targetCell).injective⟩
-
-------------------------------------------------------------------------------------------------------------------------
 --                                          insertLastAt, insertLast, ...                                             --
 ------------------------------------------------------------------------------------------------------------------------
 
@@ -443,150 +69,150 @@ theorem insertLastAt_nonempty {n : ℕ} (split : Split n) (targetCell : Cell n)
   : (split.insertLastAt targetCell).Nonempty
     := by simp [insertLastAt]
 
--- TODO: Can we simplify this proof?
-theorem insertLastAt_empty_not_mem_of_empty_not_mem
-  {n : ℕ} (split : Split n) (targetCell : Cell n) (h : ∅ ∉ split) : ∅ ∉ split.insertLastAt targetCell := by
-    simp [insertLastAt]
-    intro h_empty_elem
-    cases h_empty_elem with
-      | inl h_elem_insertLast =>
-        have := Cell.insertLast_nonempty targetCell
-        -- TODO: There has to be an easier way to show Set.Nonempty x → ∅ = x → False
-        rw [← h_elem_insertLast] at this
-        cases this with
-          | intro x h_x_elem_empty =>
-            have := Set.mem_empty_iff_false x
-            apply this.mp
-            exact h_x_elem_empty
-      | inr h_elem_removeCell =>
-        simp [removeCell] at h_elem_removeCell
-        have := Set.diff_subset split {targetCell}
-        have h_empty_not_mem_diff := Set.not_mem_subset this h
-        have h_empty_mem_diff := (castSucc_empty_elem_iff (split \ {targetCell})).mp h_elem_removeCell
-        contradiction
+-- -- TODO: Can we simplify this proof?
+-- theorem insertLastAt_empty_not_mem_of_empty_not_mem
+--   {n : ℕ} (split : Split n) (targetCell : Cell n) (h : ∅ ∉ split) : ∅ ∉ split.insertLastAt targetCell := by
+--     simp [insertLastAt]
+--     intro h_empty_elem
+--     cases h_empty_elem with
+--       | inl h_elem_insertLast =>
+--         have := Cell.insertLast_nonempty targetCell
+--         -- TODO: There has to be an easier way to show Set.Nonempty x → ∅ = x → False
+--         rw [← h_elem_insertLast] at this
+--         cases this with
+--           | intro x h_x_elem_empty =>
+--             have := Set.mem_empty_iff_false x
+--             apply this.mp
+--             exact h_x_elem_empty
+--       | inr h_elem_removeCell =>
+--         simp [removeCell] at h_elem_removeCell
+--         have := Set.diff_subset split {targetCell}
+--         have h_empty_not_mem_diff := Set.not_mem_subset this h
+--         have h_empty_mem_diff := (castSucc_empty_elem_iff (split \ {targetCell})).mp h_elem_removeCell
+--         contradiction
 
-theorem insertLastAt_is_disjoint_insert {n : ℕ} (split : Split n) (targetCell : Cell n)
-  : Disjoint {targetCell.insertLast} (split.removeCell targetCell).castSucc := by
-    apply disjoint_iff.mpr
-    simp [removeCell, castSucc, Fin.castSucc]
-    intro cell _ _
-    have h_k : ¬ (∀ (x : Fin (n + 1)), x ∈ cell.castSucc ↔ x ∈ targetCell.insertLast) := by
-      simp [not_iff]
-      exists (Fin.last n)
-      constructor
-      · intro
-        simp [Cell.insertLast]
-      · intro
-        apply Set.disjoint_singleton_left.mp
-        exact Cell.insertLast_is_disjoint_insert cell
-    have := Set.ext_iff (s := cell.castSucc) (t := targetCell.insertLast)
-    exact (not_congr this).mpr h_k
+-- theorem insertLastAt_is_disjoint_insert {n : ℕ} (split : Split n) (targetCell : Cell n)
+--   : Disjoint {targetCell.insertLast} (split.removeCell targetCell).castSucc := by
+--     apply disjoint_iff.mpr
+--     simp [removeCell, castSucc, Fin.castSucc]
+--     intro cell _ _
+--     have h_k : ¬ (∀ (x : Fin (n + 1)), x ∈ cell.castSucc ↔ x ∈ targetCell.insertLast) := by
+--       simp [not_iff]
+--       exists (Fin.last n)
+--       constructor
+--       · intro
+--         simp [Cell.insertLast]
+--       · intro
+--         apply Set.disjoint_singleton_left.mp
+--         exact Cell.insertLast_is_disjoint_insert cell
+--     have := Set.ext_iff (s := cell.castSucc) (t := targetCell.insertLast)
+--     exact (not_congr this).mpr h_k
 
--- Helper prop
-def InSplitInsertLastAtAndContainsLast {n : ℕ} (split : Split n) (targetCell : Cell n) (cell : Cell (n + 1)) : Prop
-  := cell ∈ split.insertLastAt targetCell ∧ Fin.last n ∈ cell
+-- -- Helper prop
+-- def InSplitInsertLastAtAndContainsLast {n : ℕ} (split : Split n) (targetCell : Cell n) (cell : Cell (n + 1)) : Prop
+--   := cell ∈ split.insertLastAt targetCell ∧ Fin.last n ∈ cell
 
-theorem exists_contains_last {n : ℕ} (split : Split n) (targetCell : Cell n)
-  : ∃ (cell : Cell (n + 1)), InSplitInsertLastAtAndContainsLast split targetCell cell := by
-    simp [InSplitInsertLastAtAndContainsLast, insertLastAt, Set.insert, Cell.insertLast]
+-- theorem exists_contains_last {n : ℕ} (split : Split n) (targetCell : Cell n)
+--   : ∃ (cell : Cell (n + 1)), InSplitInsertLastAtAndContainsLast split targetCell cell := by
+--     simp [InSplitInsertLastAtAndContainsLast, insertLastAt, Set.insert, Cell.insertLast]
 
-theorem unique_contains_last {n : ℕ} (split : Split n) (targetCell : Cell n)
-  : ∀ (cell₁ cell₂ : Cell (n + 1)), InSplitInsertLastAtAndContainsLast split targetCell cell₁ → InSplitInsertLastAtAndContainsLast split targetCell cell₂ → cell₁ = cell₂ := by
-    intros cell₁ cell₂ h₁ h₂
-    simp [InSplitInsertLastAtAndContainsLast, insertLastAt, Set.insert] at *
-    -- TODO: Factor out into lemma to not have to repeat this stuff
-    have h_cell₁ : cell₁ = targetCell.insertLast := by
-      have h_not_in_right : cell₁ ∉ (split.removeCell targetCell).castSucc := by
-        -- TODO: Maybe we can do this without by_contra (since it isn't constructive is it?)
-        by_contra h_in_right
-        have h_last_not_mem := last_not_mem_of_mem_removeCell_castSucc split targetCell cell₁ h_in_right
-        have h_last_mem := h₁.right
-        contradiction
-      apply (or_iff_left (a := cell₁ = targetCell.insertLast) (b := cell₁ ∈ (split.removeCell targetCell).castSucc) h_not_in_right).mp
-      exact h₁.left
-    have h_cell₂ : cell₂ = targetCell.insertLast := by
-      have h_not_in_right : cell₂ ∉ (split.removeCell targetCell).castSucc := by
-        by_contra h_in_right
-        have h_last_not_mem := last_not_mem_of_mem_removeCell_castSucc split targetCell cell₂ h_in_right
-        have h_last_mem := h₂.right
-        contradiction
-      apply (or_iff_left (a := cell₂ = targetCell.insertLast) (b := cell₂ ∈ (split.removeCell targetCell).castSucc) h_not_in_right).mp
-      exact h₂.left
-    rw [h_cell₁, h_cell₂]
+-- theorem unique_contains_last {n : ℕ} (split : Split n) (targetCell : Cell n)
+--   : ∀ (cell₁ cell₂ : Cell (n + 1)), InSplitInsertLastAtAndContainsLast split targetCell cell₁ → InSplitInsertLastAtAndContainsLast split targetCell cell₂ → cell₁ = cell₂ := by
+--     intros cell₁ cell₂ h₁ h₂
+--     simp [InSplitInsertLastAtAndContainsLast, insertLastAt, Set.insert] at *
+--     -- TODO: Factor out into lemma to not have to repeat this stuff
+--     have h_cell₁ : cell₁ = targetCell.insertLast := by
+--       have h_not_in_right : cell₁ ∉ (split.removeCell targetCell).castSucc := by
+--         -- TODO: Maybe we can do this without by_contra (since it isn't constructive is it?)
+--         by_contra h_in_right
+--         have h_last_not_mem := last_not_mem_of_mem_removeCell_castSucc split targetCell cell₁ h_in_right
+--         have h_last_mem := h₁.right
+--         contradiction
+--       apply (or_iff_left (a := cell₁ = targetCell.insertLast) (b := cell₁ ∈ (split.removeCell targetCell).castSucc) h_not_in_right).mp
+--       exact h₁.left
+--     have h_cell₂ : cell₂ = targetCell.insertLast := by
+--       have h_not_in_right : cell₂ ∉ (split.removeCell targetCell).castSucc := by
+--         by_contra h_in_right
+--         have h_last_not_mem := last_not_mem_of_mem_removeCell_castSucc split targetCell cell₂ h_in_right
+--         have h_last_mem := h₂.right
+--         contradiction
+--       apply (or_iff_left (a := cell₂ = targetCell.insertLast) (b := cell₂ ∈ (split.removeCell targetCell).castSucc) h_not_in_right).mp
+--       exact h₂.left
+--     rw [h_cell₁, h_cell₂]
 
--- NOTE: This can be used in insertLast'_produces_partitions
-theorem insertLastAt_unique_cell_last_mem {n : ℕ} (split : Split n) (targetCell : Cell n)
-  : ∃! (cell : Cell (n + 1)), InSplitInsertLastAtAndContainsLast split targetCell cell
-    := exists_unique_of_exists_of_unique (exists_contains_last split targetCell) (unique_contains_last split targetCell)
+-- -- NOTE: This can be used in insertLast'_produces_partitions
+-- theorem insertLastAt_unique_cell_last_mem {n : ℕ} (split : Split n) (targetCell : Cell n)
+--   : ∃! (cell : Cell (n + 1)), InSplitInsertLastAtAndContainsLast split targetCell cell
+--     := exists_unique_of_exists_of_unique (exists_contains_last split targetCell) (unique_contains_last split targetCell)
 
-theorem insertLastAt_castSucc_mem_of_mem_of_ne_targetCell
-    {n : ℕ}
-    {split : Split n}
-    {targetCell : Cell n}
-    {cell : Cell n}
-    (h_mem : cell ∈ split)
-    (h_ne : cell ≠ targetCell)
-  : cell.castSucc ∈ split.insertLastAt targetCell := by
-    simp [insertLastAt, Set.insert, Split,castSucc]
-    right
-    exists cell
+-- theorem insertLastAt_castSucc_mem_of_mem_of_ne_targetCell
+--     {n : ℕ}
+--     {split : Split n}
+--     {targetCell : Cell n}
+--     {cell : Cell n}
+--     (h_mem : cell ∈ split)
+--     (h_ne : cell ≠ targetCell)
+--   : cell.castSucc ∈ split.insertLastAt targetCell := by
+--     simp [insertLastAt, Set.insert, Split,castSucc]
+--     right
+--     exists cell
 
--- TODO: Maybe we can find a better name yet (it's alright, but not totally satisfactory).
--- TODO: Do we even need this if we have the version below?
-def insertLast {n : ℕ} (split : Split n) : Set (Split (n + 1))
-  := {split.insertLastAt cell | cell ∈ split.insert ∅}
+-- -- TODO: Maybe we can find a better name yet (it's alright, but not totally satisfactory).
+-- -- TODO: Do we even need this if we have the version below?
+-- def insertLast {n : ℕ} (split : Split n) : Set (Split (n + 1))
+--   := {split.insertLastAt cell | cell ∈ split.insert ∅}
 
-theorem insertLastAt_mapsTo {n : ℕ} (split : Split n)
-  : Set.MapsTo split.insertLastAt (split.insert ∅) split.insertLast := by
-    simp [Set.MapsTo, insertLast]
-    intro cell cell_mem_split
-    exists cell
+-- theorem insertLastAt_mapsTo {n : ℕ} (split : Split n)
+--   : Set.MapsTo split.insertLastAt (split.insert ∅) split.insertLast := by
+--     simp [Set.MapsTo, insertLast]
+--     intro cell cell_mem_split
+--     exists cell
 
--- TODO: Use insertLastAt_mapsTo here
-theorem insertLastAt_surjOn {n : ℕ} (split : Split n)
-  : Set.SurjOn split.insertLastAt (split.insert ∅) split.insertLast := by
-    simp [Set.SurjOn, insertLast, Set.image]
-    intro cell cell_mem_split'
-    exists cell
+-- -- TODO: Use insertLastAt_mapsTo here
+-- theorem insertLastAt_surjOn {n : ℕ} (split : Split n)
+--   : Set.SurjOn split.insertLastAt (split.insert ∅) split.insertLast := by
+--     simp [Set.SurjOn, insertLast, Set.image]
+--     intro cell cell_mem_split'
+--     exists cell
 
-theorem insertLastAt_bijOn {n : ℕ} (split : Split n)
-  : Set.BijOn split.insertLastAt (split.insert ∅) split.insertLast := by
-    split_ands
-    · exact insertLastAt_mapsTo split
-    · exact insertLastAt_injOn split
-    · exact insertLastAt_surjOn split
+-- theorem insertLastAt_bijOn {n : ℕ} (split : Split n)
+--   : Set.BijOn split.insertLastAt (split.insert ∅) split.insertLast := by
+--     split_ands
+--     · exact insertLastAt_mapsTo split
+--     · exact insertLastAt_injOn split
+--     · exact insertLastAt_surjOn split
 
-theorem insertLast_nonempty_of_mem
-  {n : ℕ}
-  {split : Split n}
-  {split' : Split (n + 1)}
-  (h : split' ∈ insertLast split)
-  : split'.Nonempty := by
-    simp [insertLast] at h
-    cases h with
-      | intro cell h_cell =>
-        rw [← h_cell.right]
-        exact insertLastAt_nonempty _ _
+-- theorem insertLast_nonempty_of_mem
+--   {n : ℕ}
+--   {split : Split n}
+--   {split' : Split (n + 1)}
+--   (h : split' ∈ insertLast split)
+--   : split'.Nonempty := by
+--     simp [insertLast] at h
+--     cases h with
+--       | intro cell h_cell =>
+--         rw [← h_cell.right]
+--         exact insertLastAt_nonempty _ _
 
-def insertLast' {n : ℕ} (h : n > 0) (split : Split (n - 1)) : Set (Split n)
-  := cast (Nat.sub_add_cancel h) '' split.insertLast
+-- def insertLast' {n : ℕ} (h : n > 0) (split : Split (n - 1)) : Set (Split n)
+--   := cast (Nat.sub_add_cancel h) '' split.insertLast
 
-theorem insertLast'_nonempty_of_mem
-  {n : ℕ}
-  {h : n > 0}
-  {split : Split (n - 1)}
-  {split' : Split n}
-  (h : split' ∈ insertLast' h split)
-  : split'.Nonempty := by
-    simp [insertLast'] at h
-    cases h with
-      | intro split'' h_split'' =>
-        rw [← h_split''.right]
-        have h_split''_nonempty : split''.Nonempty := insertLast_nonempty_of_mem h_split''.left
-        simp [cast_nonempty_iff, h_split''_nonempty]
+-- theorem insertLast'_nonempty_of_mem
+--   {n : ℕ}
+--   {h : n > 0}
+--   {split : Split (n - 1)}
+--   {split' : Split n}
+--   (h : split' ∈ insertLast' h split)
+--   : split'.Nonempty := by
+--     simp [insertLast'] at h
+--     cases h with
+--       | intro split'' h_split'' =>
+--         rw [← h_split''.right]
+--         have h_split''_nonempty : split''.Nonempty := insertLast_nonempty_of_mem h_split''.left
+--         simp [cast_nonempty_iff, h_split''_nonempty]
 
--- TODO: Probably fix this by mapping Finset.toSet
-def IsPartition {n : ℕ} (split : Split n) : Prop
-  := Setoid.IsPartition split
+-- -- TODO: Probably fix this by mapping Finset.toSet
+-- def IsPartition {n : ℕ} (split : Split n) : Prop
+--   := Setoid.IsPartition split
 
 end Split
