TheoremsAboutAlgorithms/Partitions/WithFinset/Split/UpwardDownward.lean
@@ -1,0 +1,356 @@
+import TheoremsAboutAlgorithms.Partitions.WithFinset.Defs
+import TheoremsAboutAlgorithms.Partitions.WithFinset.Split.Basic
+
+namespace Split
+
+-- TODO: Group theorems below in anonymous sections where we can then also e.g. set `split`, `targetCell` etc once all
+--       theorems in the section use them.
+variable {n : ℕ}
+
+------------------------------------------------------------------------------------------------------------------------
+--                          Embeddings between split and split.insertLastAt targetCell                                --
+------------------------------------------------------------------------------------------------------------------------
+
+-- What we want and define here are functions `f` and `g` (which will have more descriptive names below) such that
+--
+--    `f : split → split.insertLastAt targetCell`
+--    `g : split.insertLastAt targetCell → split`
+--
+-- and `f ∘ g = id` and `g ∘ f = id`. We want to define them as follows:
+--
+--    `f := if cell = targetCell then cell.insertLast else cell.castSucc`
+--    `g := if cell = targetCell.insertLast then targetCell else cell.castPred`
+--
+-- To do that we need an assumption `{Fin.last _} ∉ split.insertLastAt targetCell` to be able to define `g` as above,
+-- because that has the preimage `∅` which we can't include in the domain of `f` (and therefore also not in the codomain
+-- of `g`).
+--
+-- TODO: See in the usage later if that is what we actually need. Maybe we can `split.insertEmpty` work as domain of `f`
+--       as codomain of `g` as well.
+
+-- TODO:
+--    * Theorem names and naming in general in this section are lacking, improve them!
+
+-- TODO: Make this a section and define all the common implicit arguments (`n, split, targetCell`) at the top
+theorem insertLast_mem_insertLastAt_of_eq
+    {split : Split n}
+    {targetCell cell : Cell n}
+    (cell_eq_targetCell : cell = targetCell)
+  : cell.insertLast ∈ split.insertLastAt targetCell := by
+    simp [insertLastAt]
+    left
+    rw [cell_eq_targetCell]
+
+-- TODO: How can we make this anonymous so it can be found implicitly if we have the equality hypothesis?
+--       Maybe this resource can help find the answer:
+--        https://leanprover-community.github.io/mathlib4_docs/Init/Coe.html
+--
+--      Maybe `#print toInsertLastAt` can help us find the answer.
+instance CoeDepInsertLastInsertLastAtOfEq
+    {split : Split n}
+    {targetCell cell : Cell n}
+    (cell_eq_targetCell : cell = targetCell)
+  : CoeDep (Cell (n + 1)) (cell.insertLast) (split.insertLastAt targetCell) where
+    coe := by
+      use cell.insertLast
+      exact insertLast_mem_insertLastAt_of_eq cell_eq_targetCell
+
+-- We can't have `cell : split.insertEmpty`, because `Cell.castSucc ∅` is not in fact in `split.insertLastAt`. We do
+-- however want to use this in the situation where `split` is a partition meaning that `∅ ∉ split`. We only use
+-- `partitions.insertEmpty` there the have a target for the to create `{Fin.last _}`. We probably do not need to have
+-- `insertEmptyToInsertLastAt` to go from `partition.insertEmpty` but can use just `partition` as the domain. We handle
+-- the case where `cell = ∅` separately.
+theorem castSucc_mem_insertLastAt_of_ne
+    {split : Split n}
+    {targetCell : Cell n}
+    {cell : split}
+    (cell_ne_targetCell : ↑cell ≠ targetCell)
+  : Cell.castSucc cell ∈ split.insertLastAt targetCell := by
+    simp [insertLastAt, castSucc, Cell.castSuccEmbedding, Cell.castSucc]
+    right
+    assumption
+
+-- TODO: How can we make this anonymous (like above)?
+instance CoeDepCastSuccInsertLastAtOfNe
+    {split : Split n}
+    {targetCell : Cell n}
+    {cell : split}
+    (cell_ne_targetCell : ↑cell ≠ targetCell)
+  : CoeDep (Cell (n + 1)) (Cell.castSucc cell) (split.insertLastAt targetCell) where
+    coe := by
+      use Cell.castSucc cell
+      exact castSucc_mem_insertLastAt_of_ne cell_ne_targetCell
+
+def upward
+    {split : Split n}
+    {targetCell : Cell n}
+    (cell : split)
+  : split.insertLastAt targetCell :=
+    if h : cell = targetCell
+    -- CoeDep.coe.{u, v} {α : Sort u} (x✝ : α) {β : Sort v} [self : CoeDep α x✝ β] : β
+    -- then CoeDep.coe _ (Cell.castSucc cell) _ (CoeDepInsertLastInsertLastAtOfEq h)
+    then (CoeDepInsertLastInsertLastAtOfEq h).coe
+    else (CoeDepCastSuccInsertLastAtOfNe h).coe
+
+-- TODO: Naming feels pretty imprecise here
+theorem ne_last_of_ne_insertLast_of_mem
+    {split : Split n}
+    {targetCell : Cell n}
+    {cell : split.insertLastAt targetCell}
+    (cell_ne_targetCell_insertLast : ↑cell ≠ targetCell.insertLast)
+    (x : ↑cell)
+  : ↑x ≠ Fin.last n := by
+    have cell_mem_insertLastAt := cell.property
+    simp [insertLastAt] at cell_mem_insertLastAt
+    cases cell_mem_insertLastAt with
+      | inl _ => contradiction
+      | inr cell_mem_castSucc =>
+        apply Decidable.byContradiction
+        intro x_eq_last
+        simp at x_eq_last
+        have last_mem_cell : Fin.last n ∈ (cell : Cell (n + 1)) := by
+          have := x.property;
+          rw [x_eq_last] at this;
+          exact this
+        have last_not_mem_cell := last_not_mem_of_mem_castSucc cell_mem_castSucc
+        contradiction
+
+-- TODO: Naming feels pretty imprecise here
+theorem ne_last_of_ne_insertLast
+    {split : Split n}
+    {targetCell : Cell n}
+    {cell : split.insertLastAt targetCell}
+    (cell_ne_targetCell_insertLast : ↑cell ≠ targetCell.insertLast)
+  : ∀ x ∈ (cell : Cell (n + 1)), ↑x ≠ Fin.last n := by
+    intro x x_mem_cell
+    exact ne_last_of_ne_insertLast_of_mem cell_ne_targetCell_insertLast ⟨x, x_mem_cell⟩
+
+theorem mem_castSucc_of_ne_targetCell_of_mem_castSucc_erase_targetCell
+    {split : Split n}
+    {targetCell : Cell n}
+    {cell : Cell (n + 1)}
+    (cell_mem_castSucc_erase_targetCell : cell ∈ (split.erase targetCell |> castSucc))
+  : cell ∈ split.castSucc := by
+      simp [castSucc, Cell.castSuccEmbedding] at *
+      obtain ⟨_, cell', _, _⟩ := cell_mem_castSucc_erase_targetCell
+      use cell'
+
+-- cell'_mem_split : cell' ∈ split
+-- castSucc_cell'_eq_cell : Cell.castSucc cell' = ↑cell
+-- ⊢ Cell.castPred ↑cell _ ∈ split
+theorem castPred_mem_split_of_mem_split_of_castSucc_eq_of_last_not_mem
+    {split : Split n}
+    {x : Cell n}
+    {y : Cell (n + 1)}
+    (x_mem_split : x ∈ split)
+    (castSucc_x_eq_y : Cell.castSucc x = y)
+    (last_not_mem_y : ∀ f ∈ y, f ≠ Fin.last _)
+  : Cell.castPred y last_not_mem_y ∈ split := by
+    -- See https://proofassistants.stackexchange.com/a/1063 for why we use `subst` here
+    rw [Cell.castPred_y_eq_x_of_castSucc_x_eq_y_of_forall_mem_y_ne_last castSucc_x_eq_y last_not_mem_y]
+    exact x_mem_split
+
+theorem castPred_mem_of_ne_insertLast_of_mem_castSucc
+    {split : Split n}
+    {targetCell : Cell n}
+    {cell : split.insertLastAt targetCell}
+    (cell_ne_insertLast_targetCell : ↑cell ≠ targetCell.insertLast)
+    (cell_mem_castSucc : ↑cell ∈ split.castSucc)
+  : (Cell.castPred cell) (ne_last_of_ne_insertLast cell_ne_insertLast_targetCell) ∈ split := by
+    simp [castSucc, Cell.castSuccEmbedding] at cell_mem_castSucc
+    obtain ⟨cell', cell'_mem_split, castSucc_cell'_eq_cell⟩ := cell_mem_castSucc
+    -- We use the helper because `rw` and `subst` do not work here (probably because we're coercing `cell` via `↑cell`)
+    apply castPred_mem_split_of_mem_split_of_castSucc_eq_of_last_not_mem cell'_mem_split castSucc_cell'_eq_cell
+
+theorem castPred_mem_of_mem_insertLastAt_of_ne_targetCell
+    {split : Split n}
+    {targetCell : Cell n}
+    {cell : split.insertLastAt targetCell}
+    (cell_ne_insertLast_targetCell : ↑cell ≠ targetCell.insertLast)
+  : (Cell.castPred cell) (ne_last_of_ne_insertLast cell_ne_insertLast_targetCell) ∈ split := by
+    have cell_mem_insertLastAt := cell.property
+    simp [insertLastAt] at cell_mem_insertLastAt
+    cases cell_mem_insertLastAt with
+      | inl cell_eq_targetCell_insertLast => contradiction
+      | inr cell_mem_castSucc =>
+        apply castPred_mem_of_ne_insertLast_of_mem_castSucc cell_ne_insertLast_targetCell
+        exact mem_castSucc_of_ne_targetCell_of_mem_castSucc_erase_targetCell cell_mem_castSucc
+
+instance CoeDepCastPredOfNeInsertLast
+    {split : Split n}
+    {targetCell : Cell n}
+    {cell : split.insertLastAt targetCell}
+    (cell_ne_insertLast_targetCell : ↑cell ≠ targetCell.insertLast)
+  : CoeDep (Cell n) ((Cell.castPred cell) (ne_last_of_ne_insertLast cell_ne_insertLast_targetCell)) split where
+    coe := by
+      use (Cell.castPred cell) (ne_last_of_ne_insertLast cell_ne_insertLast_targetCell)
+      exact castPred_mem_of_mem_insertLastAt_of_ne_targetCell cell_ne_insertLast_targetCell
+
+-- TODO: This should probably be defined for `cell ≠ {Fin.last _}`, we just handle that case differently, so we have the
+--       codomain equal to `toInsertLastAt`'s domain
+def downward
+    (split : Split n)
+    (targetCell : split)
+    (cell : split.insertLastAt targetCell)
+  : split :=
+    if h : cell = Cell.insertLast (targetCell : Cell n)
+    then targetCell
+    else (CoeDepCastPredOfNeInsertLast h).coe
+
+theorem castPred_x_mem_split_of_mem_split_of_castSucc_eq
+    {split : Split n}
+    {x' : Cell n}
+    {x : Cell (n + 1)}
+    (x'_mem_split : x' ∈ split)
+    (castSucc_x'_eq_x : Cell.castSucc x' = x)
+    -- TODO: Better api for the precondition, maybe as a predicate?
+    (castPred_x_preCond : ∀ f ∈ x, f ≠ Fin.last _ := by simp)
+  : Cell.castPred x castPred_x_preCond ∈ split := by
+    subst x
+    simp [Cell.castPred_castSucc_eq]
+    exact x'_mem_split
+
+-- Surjectivity
+theorem upward_surjective
+    {split : Split n}
+    (targetCell : split)
+  : Function.Surjective (@upward _ split targetCell) := by
+    intro x
+    simp [upward]
+    -- TODO: Make this work
+    -- TODO: Find a way we can use better notation than the explicit long instance name
+    -- let y := (@CoeDepInsertLastInsertLastAtOfEq n _ _ ).coe
+    cases Decidable.eq_or_ne x (CoeDepInsertLastInsertLastAtOfEq rfl).coe with
+      | inl x_eq_coe_insertLast_targetCell =>
+        exists targetCell
+        exists targetCell.property
+        split
+        · exact x_eq_coe_insertLast_targetCell.symm
+        · contradiction
+      | inr x_ne_coe_insertLast_targetCell =>
+        have x_val_ne_insertLast_targetCell : (x : Cell (n + 1)) ≠ Cell.insertLast ↑targetCell := by
+          simp [CoeDep.coe] at *
+          intro x_val_eq_insertLast_targetCell
+          have : x = (CoeDepInsertLastInsertLastAtOfEq rfl).coe := by
+            apply @Subtype.eq _ _ x _
+            exact x_val_eq_insertLast_targetCell
+          contradiction
+        -- If we use this (instead of writing out the verbose expression), this makes `castPred_h_x` appear everywhere
+        -- we would otherwise have `_` in the proof state which is ugly
+        -- let castPred_h_x := (ne_last_of_ne_insertLast x_val_ne_insertLast_targetCell)
+        -- TODO: How can we make it that we put this into the context and it is found implicitly?
+        exists Cell.castPred x (ne_last_of_ne_insertLast x_val_ne_insertLast_targetCell)
+        have castPred_x_val_mem_split : Cell.castPred x (ne_last_of_ne_insertLast x_val_ne_insertLast_targetCell) ∈ split := by
+          have x_val_mem_insertLastAt := x.property
+          simp [insertLastAt, x_val_ne_insertLast_targetCell, castSucc, Cell.castSuccEmbedding]
+            at x_val_mem_insertLastAt
+          obtain ⟨_, x', x'_mem_split, castSucc_x'_eq_x_val⟩ := x_val_mem_insertLastAt
+          exact castPred_x_mem_split_of_mem_split_of_castSucc_eq x'_mem_split castSucc_x'_eq_x_val _
+        exists castPred_x_val_mem_split
+        split
+        · case _ castPred_x_val_eq_targetCell_val =>
+          have x_val_mem_insertLastAt := x.property
+          simp [insertLastAt, x_val_ne_insertLast_targetCell, castSucc, Cell.castSuccEmbedding]
+            at x_val_mem_insertLastAt
+          obtain ⟨x_val_ne_castSucc_targetCell, _⟩ := x_val_mem_insertLastAt
+          have := Cell.eq_castSucc_of_castPred_eq _ castPred_x_val_eq_targetCell_val
+          contradiction
+        · case _ castPred_x_val_ne_insertLast_targetCell =>
+          simp [CoeDep.coe]
+          apply Subtype.eq
+          simp [Cell.castSucc_castPred_eq]
+
+-- Inverses
+
+theorem left_inverse_downward_upward
+    {split : Split n}
+    (targetCell : split)
+  : Function.LeftInverse (@downward _ split targetCell) (@upward _ split targetCell) := by
+    intro x
+    simp [upward, downward]
+    split
+    · case _ x_eq_targetCell =>
+      split
+      · apply Subtype.eq
+        exact x_eq_targetCell.symm
+      · case _ insertLast_x_ne_insertLast_targetCell =>
+        simp [CoeDep.coe] at insertLast_x_ne_insertLast_targetCell
+        -- TODO: There has to be a better way to get f x = f y from x = y
+        have : Cell.insertLast ↑x = Cell.insertLast (targetCell : Cell n) := by
+          have : Cell.insertLast ↑x = Cell.insertLast (x : Cell n) := by rfl
+          rw (config := {occs := .pos [2]}) [x_eq_targetCell] at this
+          exact this
+        contradiction
+    · case _ x_ne_targetCell_insertLast =>
+      split
+      · case _ castSucc_x_eq_insertLast_targetCell =>
+        simp [CoeDep.coe] at castSucc_x_eq_insertLast_targetCell
+        have := Cell.castSucc_x_ne_insertLast_y (x : Cell n) (targetCell : Cell n)
+        contradiction
+      · case _ castSucc_x_ne_insertLast_targetCell =>
+        simp [CoeDep.coe, x_ne_targetCell_insertLast]
+        apply Subtype.eq
+        simp
+        apply Cell.castPred_y_eq_x_of_castSucc_x_eq_y_of_forall_mem_y_ne_last rfl
+
+theorem right_inverse_downward_upward
+    {split : Split n}
+    (targetCell : split)
+  : Function.RightInverse (@downward _ split targetCell) (@upward _ split targetCell) := by
+    apply Function.LeftInverse.rightInverse_of_surjective
+    · apply left_inverse_downward_upward
+    · apply upward_surjective
+
+theorem left_inverse_upward_downward
+    {split : Split n}
+    (targetCell : split)
+  : Function.LeftInverse (@upward _ split targetCell) (@downward _ split targetCell) := by
+    apply Function.RightInverse.leftInverse
+    apply right_inverse_downward_upward
+
+theorem right_inverse_upward_downward
+    {split : Split n}
+    (targetCell : split)
+  : Function.RightInverse (@upward _ split targetCell) (@downward _ split targetCell) := by
+    apply Function.LeftInverse.rightInverse
+    apply left_inverse_downward_upward
+
+theorem upward_injective
+    {split : Split n}
+    (targetCell : split)
+  : Function.Injective (@upward _ split targetCell)
+    := Function.LeftInverse.injective (left_inverse_downward_upward targetCell)
+
+theorem upward_bijective
+    {split : Split n}
+    (targetCell : split)
+  : Function.Bijective (@upward _ split targetCell) := by
+    constructor
+    · apply upward_injective
+    · apply upward_surjective
+
+theorem downward_bijective
+    {split : Split n}
+    (targetCell : split)
+  : Function.Bijective (@downward _ split targetCell) := by
+    apply Function.bijective_iff_has_inverse.mpr
+    exists upward
+    constructor
+    · apply left_inverse_upward_downward
+    · apply right_inverse_upward_downward
+
+-- Injectivity, embeddings
+
+def upwardEmbedding
+    {split : Split n}
+    (targetCell : split)
+  : Function.Embedding split (split.insertLastAt targetCell) :=
+    ⟨upward, upward_injective targetCell⟩
+
+def downwardEmbedding
+    {split : Split n}
+    (targetCell : split)
+  : Function.Embedding (split.insertLastAt targetCell) split :=
+    ⟨downward split targetCell, (downward_bijective targetCell).injective⟩
+
+end Split
